DeBruijnSSA/BinSyntax/Effect.lean
@@ -1,0 +1,46 @@
+import Discretion.Wk.Order
+
+import DeBruijnSSA.BinSyntax.Syntax.Definitions
+import DeBruijnSSA.InstSet
+
+namespace BinSyntax
+
+variable [Φ : EffectSet φ ε] [Bot ε] [Sup ε]
+
+/-- Infer the effect of a term -/
+def Term.effect (Γ : ℕ → ε) : Term φ → ε
+  | var n => Γ n
+  | op f e => Φ.effect f ⊔ e.effect Γ
+  | pair a b => a.effect Γ ⊔ b.effect Γ
+  | inl a => a.effect Γ
+  | inr b => b.effect Γ
+  | abort e => e.effect Γ
+  | unit => ⊥
+
+/-- Infer the effect of a body -/
+def Body.effect (Γ : ℕ → ε) : Body φ → ε
+  | nil => ⊥
+  | let1 e b => e.effect Γ ⊔ b.effect (Nat.liftBot Γ)
+  | let2 e b => e.effect Γ ⊔ b.effect (Nat.liftnBot 2 Γ)
+
+-- TODO: this is currently asserting that the arguments to `case` and `br` always have effect `⊥`!
+
+/-- Infer the effect of a `BBRegion`, _without_ taking control-flow into account -/
+def BBRegion.effect (Γ : ℕ → ε) : BBRegion φ → ε
+  | cfg β _ G => β.body.effect Γ ⊔ Fin.sup (λi => (G i).effect (Nat.liftnBot β.body.num_defs Γ))
+
+/-- Infer the effect of a `TRegion`, _without_ taking control-flow into account -/
+def TRegion.effect (Γ : ℕ → ε) : TRegion φ → ε
+  | let1 e r => e.effect Γ ⊔ r.effect (Nat.liftBot Γ)
+  | let2 e r => e.effect Γ ⊔ r.effect (Nat.liftnBot 2 Γ)
+  | cfg _ _ G => Fin.sup (λi => (G i).effect Γ)
+
+/-- Infer the effect of a `Region`, _without_ taking control-flow into account -/
+def Region.effect (Γ : ℕ → ε) : Region φ → ε
+  | br _ _ => ⊥
+  | let1 e r => e.effect Γ ⊔ r.effect (Nat.liftBot Γ)
+  | let2 e r => e.effect Γ ⊔ r.effect (Nat.liftnBot 2 Γ)
+  | case _ s t => s.effect Γ ⊔ t.effect Γ
+  | cfg β _ G => β.effect Γ ⊔ Fin.sup (λi => (G i).effect Γ)
+
+end BinSyntax
